TODO: assert (forall k, l: int :: lo <= k && k < l && l <= hi ==> perm[k] != perm[l]);

bucketSort.bpl
@@ -1,6 +1,8 @@
 const N: int;
 axiom 0 <= N;
 
+type Tuple t1 t1;
+
 // Declare a map from integers to integers.
 // 'a' should be treated as an array of 'N' elements, indexed from 0 to N-1
 var a: [int]int;
@@ -54,6 +56,10 @@ procedure bucketSort(lo : int, hi : int) returns (perm: [int]int)
   
   //bucket permutations
   var perm0, perm1, perm2 : [int]int;
+  var permAtoB0 : [int]int;
+  var permAtoB1 : [int]int;
+  var permAtoB2 : [int]int;
+  var permA : [int]int;
 
   var b0, b0_sorted, b1, b1_sorted, b2, b2_sorted: [int]int;
   
@@ -76,25 +82,92 @@ procedure bucketSort(lo : int, hi : int) returns (perm: [int]int)
     invariant(forall e:int :: (e >= 0 && e < b0_i) ==> (b0[e] < -1*N));
     invariant(forall e:int :: (e >= 0 && e < b1_i) ==> (b1[e] >= -1*N && b1[e] < N));
     invariant(forall e:int :: (e >= 0 && e < b2_i) ==> (b2[e] >= N));
+    
+    //permAtoB holds the mapping of elements from A onto the buckets
+    invariant(forall e:int :: (e >= 0 && e < b0_i) ==> (b0[e] == a[permAtoB0[e]]));
+    invariant(forall e:int :: (e >= 0 && e < b1_i) ==> (b1[e] == a[permAtoB1[e]]));
+    invariant(forall e:int :: (e >= 0 && e < b2_i) ==> (b2[e] == a[permAtoB2[e]]));
+    
+    invariant (forall k: int :: 0 <= k && k < b0_i ==> lo <= permAtoB0[k] && permAtoB0[k] <= hi);
+    invariant (forall k: int :: 0 <= k && k < b1_i ==> lo <= permAtoB1[k] && permAtoB1[k] <= hi);
+    invariant (forall k: int :: 0 <= k && k < b2_i ==> lo <= permAtoB2[k] && permAtoB2[k] <= hi);
   {
     //add a[i] to correct bucket
     if(a[i] < bound_1){
       if(a[i] < bound_0){
         b0[b0_i] := a[i];
+        permAtoB0[b0_i] := i;
+        
         b0_i := b0_i + 1;
       }
       else{
         b1[b1_i] := a[i];
+        permAtoB1[b1_i] := i;
+        
         b1_i := b1_i + 1;
       }
     }
     else{
       b2[b2_i] := a[i];
+      permAtoB2[b2_i] := i;
+        
       b2_i := b2_i + 1;
     }
     i := i + 1;
   }
-
+  
+  assert(i == hi+1);
+  assert(b0_i + b1_i + b2_i == hi-lo + 1);
+  
+  i := 0;
+  while(i < b0_i)
+    invariant (i >= 0 && i <= b0_i);
+    invariant(forall e:int :: (e >= 0 && e < i) ==> (b0[e] == a[permA[e]]));
+    invariant (forall k: int :: 0 <= k && k < i ==> lo <= permA[k] && permA[k] <= hi);
+  {
+    permA[i] := permAtoB0[i];
+    i := i + 1;
+  }
+  
+  assert(i == b0_i);
+  assert(forall e:int :: (e >= 0 && e < b0_i) ==> (b0[e] == a[permA[e]]));
+  
+  i := 0;
+  while(i < b1_i)
+    invariant(i >= 0 && i <= b1_i);
+    invariant(forall e:int :: (e >= 0 && e < b0_i) ==> (b0[e] == a[permA[e]]));
+    invariant(forall e:int :: (e >= 0 && e < i) ==> (b1[e] == a[permA[e + b0_i]]));
+    invariant (forall k: int :: 0 <= k && k < b0_i ==> lo <= permA[k] && permA[k] <= hi);
+    invariant (forall k: int :: b0_i <= k && k < i+b0_i ==> lo <= permA[k] && permA[k] <= hi);
+  {
+    permA[i+b0_i] := permAtoB1[i];
+    i := i + 1;
+  }
+  
+  assert (i == b1_i);
+  assert(forall e:int :: (e >= 0 && e < b0_i) ==> (b0[e] == a[permA[e]]));
+  assert(forall e:int :: (e >= 0 && e < b1_i) ==> (b1[e] == a[permA[e + b0_i]]));
+  
+  i := 0;
+  while(i < b2_i)
+    invariant(i >= 0 && i <= b2_i);
+    invariant(forall e:int :: (e >= 0 && e < b0_i) ==> (b0[e] == a[permA[e]]));
+    invariant(forall e:int :: (e >= 0 && e < b1_i) ==> (b1[e] == a[permA[e + b0_i]]));
+    invariant(forall e:int :: (e >= 0 && e < i) ==> (b2[e] == a[permA[e + b0_i + b1_i]]));
+    invariant (forall k: int :: 0 <= k && k < b0_i ==> lo <= permA[k] && permA[k] <= hi);
+    invariant (forall k: int :: b0_i <= k && k < b1_i+b0_i ==> lo <= permA[k] && permA[k] <= hi);
+    invariant (forall k: int :: b0_i + b1_i <= k && k < b0_i + b1_i + i ==> lo <= permA[k] && permA[k] <= hi);
+  {
+    permA[i + b0_i + b1_i] := permAtoB2[i];
+    i := i + 1;
+  }
+  
+  assert(i == b2_i);
+  assert(forall e:int :: (e >= 0 && e < b0_i) ==> (b0[e] == a[permA[e]]));
+  assert(forall e:int :: (e >= 0 && e < b1_i) ==> (b1[e] == a[permA[e + b0_i]]));
+  assert(forall e:int :: (e >= 0 && e < b2_i) ==> (b2[e] == a[permA[e + b0_i + b1_i]]));
+  
+  
   // index mapping from bucket indexes to array indexes 
   off_b0 := lo + b0_i; // end index of bucket0 in a (exclusive)
   off_b1 := lo + b0_i + b1_i; // end index of bucket1 in a (exclusive)
@@ -104,15 +177,54 @@ procedure bucketSort(lo : int, hi : int) returns (perm: [int]int)
   if(b0_i > 0) { call b0_sorted, perm0 := quickSort(b0, 0, b0_i-1); }
   if(b1_i > 0) { call b1_sorted, perm1 := quickSort(b1, 0, b1_i-1); }
   if(b2_i > 0) { call b2_sorted, perm2 := quickSort(b2, 0, b2_i-1); }
+  
+  assert(forall e:int :: (e >= 0 && e < b0_i) ==> (b0[e] == a[permA[e]]));
+  assert(forall e:int :: (e >= 0 && e < b1_i) ==> (b1[e] == a[permA[e + b0_i]]));
+  assert(forall e:int :: (e >= 0 && e < b2_i) ==> (b2[e] == a[permA[e + b0_i + b1_i]]));
+  
+  assert(forall e:int :: (e >= 0 && e < b0_i) ==> (b0_sorted[e] == b0[perm0[e]]));
+  assert(forall e:int :: (e >= 0 && e < b1_i) ==> (b1_sorted[e] == b1[perm1[e]]));
+  assert(forall e:int :: (e >= 0 && e < b2_i) ==> (b2_sorted[e] == b2[perm2[e]]));
+  
+  assert(forall e:int :: (e >= 0 && e < b0_i) ==> (b0_sorted[e] == old(a[permA[perm0[e]]])));
+  assert(forall e:int :: (e >= 0 && e < b1_i) ==> (b1_sorted[e] == old(a[permA[perm1[e] + b0_i]])));
+  assert(forall e:int :: (e >= 0 && e < b2_i) ==> (b2_sorted[e] == old(a[permA[perm2[e] + b0_i + b1_i]])));
+  
+  assert(forall e:int :: (e >= lo && e < lo + b0_i) ==> (b0_sorted[e-lo] == old(a[permA[perm0[e-lo]]])));
+  assert(forall e:int :: (e >= lo && e < lo + b1_i) ==> (b1_sorted[e-lo] == old(a[permA[perm1[e-lo] + b0_i]])));
+  assert(forall e:int :: (e >= lo && e < lo + b2_i) ==> (b2_sorted[e-lo] == old(a[permA[perm2[e-lo] + b0_i + b1_i]])));
+  
+  assert(forall e:int :: (e >= lo && e <= hi) ==> (
+    (e < b0_i ==> b0_sorted[e-lo] == old(a[permA[perm0[e-lo]]]))
+    &&
+    (e >= b0_i && e < b0_i + b1_i ==> (b1_sorted[e-b0_i] == old(a[permA[perm1[e-b0_i] + b0_i]])))
+    &&
+    (e >= b0_i + b1_i && e < b0_i + b1_i + b2_i ==> b2_sorted[e-b0_i-b1_i] == old(a[permA[perm2[e-b0_i-b1_i] + b0_i + b1_i]]))
+    )
+  );
+  
+   assert (forall k: int :: 0 <= k && k < b0_i ==> lo <= permA[k] && permA[k] <= hi);
+    assert (forall k: int :: b0_i <= k && k < b1_i+b0_i ==> lo <= permA[k] && permA[k] <= hi);
+    assert (forall k: int :: b0_i + b1_i <= k && k < b0_i + b1_i + b2_i ==> lo <= permA[k] && permA[k] <= hi);
+   assert (forall k: int :: 0 <= k && k <= hi-lo ==> lo <= permA[k] && permA[k] <= hi);
+  //assert(forall e:int :: (e >= lo && e <= hi) ==> ());
 
   i := lo;
   while(i < off_b0)
     // bucket values are copied to a
     invariant (forall k: int :: lo <= k && k < i ==> a[k] == b0_sorted[k-lo]);
+    invariant (forall k: int :: lo <= k && k < i ==> a[k] == old(a[perm[k]]));
+    invariant (forall k: int :: lo <= k && k < i ==> lo <= perm[k] && perm[k] <= hi);
   {
     a[i] := b0_sorted[i-lo];
+    perm[i] := permA[perm0[i-lo]];
     i := i + 1;
   }
+
+  assert(forall e:int :: (e >= lo && e <= hi) ==> (
+      (e < off_b0 ==> a[e] == old(a[perm[e]]))
+    )
+  );
 
   // copy back elements from bucket to array
   i := off_b0;
@@ -123,8 +235,15 @@ procedure bucketSort(lo : int, hi : int) returns (perm: [int]int)
     invariant (forall k: int :: lo <= k && k < off_b0 ==> a[k] == b0_sorted[k-lo]);
     // bucket values are copied to a
     invariant (forall k: int :: off_b0 <= k && k < i ==> a[k] == b1_sorted[k-off_b0]);
+    
+    //permutation
+    invariant (forall k: int :: lo <= k && k < off_b0 ==> a[k] == old(a[perm[k]]));
+    invariant (forall k: int :: off_b0 <= k && k < i ==> a[k] == old(a[perm[k]]));
+    invariant (forall k: int :: lo <= k && k < off_b0 ==> lo <= perm[k] && perm[k] <= hi);
+    invariant (forall k: int :: off_b0 <= k && k < i ==> lo <= perm[k] && perm[k] <= hi);
   {
-    a[i] := b1_sorted[i-off_b0];   
+    a[i] := b1_sorted[i-off_b0];
+    perm[i] := permA[perm1[i-b0_i-lo] + b0_i];
     i := i + 1;
   }
   
@@ -137,8 +256,17 @@ procedure bucketSort(lo : int, hi : int) returns (perm: [int]int)
     invariant (forall k: int :: off_b0 <= k && k < off_b1 ==> a[k] == b1_sorted[k-off_b0]);
     // bucket values are copied to a
     invariant (forall k: int :: off_b1 <= k && k < i ==> a[k] == b2_sorted[k-off_b1]);
+    
+    //permutation
+    invariant (forall k: int :: lo <= k && k < off_b0 ==> a[k] == old(a[perm[k]]));
+    invariant (forall k: int :: off_b0 <= k && k < off_b1 ==> a[k] == old(a[perm[k]]));
+    invariant (forall k: int :: off_b1 <= k && k < i ==> a[k] == old(a[perm[k]]));
+    invariant (forall k: int :: lo <= k && k < off_b0 ==> lo <= perm[k] && perm[k] <= hi);
+    invariant (forall k: int :: off_b0 <= k && k < off_b1 ==> lo <= perm[k] && perm[k] <= hi);
+    invariant (forall k: int :: off_b1 <= k && k < i ==> lo <= perm[k] && perm[k] <= hi);
   {
-    a[i] := b2_sorted[i-off_b1];   
+    a[i] := b2_sorted[i-off_b1];
+    perm[i] := permA[perm2[i-b0_i-b1_i-lo] + b0_i + b1_i];
     i := i + 1;
   }
 
@@ -155,8 +283,8 @@ procedure bucketSort(lo : int, hi : int) returns (perm: [int]int)
   // assert (forall k, l: int ::     lo <= k && k <= l && l <= hi ==> a[k] <= a[l]);
 
   // TODO we still need to construct a permutation and prove these properties
-  assume (forall k: int :: lo <= k && k <= hi ==> lo <= perm[k] && perm[k] <= hi);
-  assume (forall k, l: int :: lo <= k && k < l && l <= hi ==> perm[k] != perm[l]);
-  assume (forall k: int :: lo <= k && k <= hi ==> a[k] == old(a)[perm[k]]);
+  assert (forall k: int :: lo <= k && k <= hi ==> lo <= perm[k] && perm[k] <= hi);
+  assert (forall k, l: int :: lo <= k && k < l && l <= hi ==> perm[k] != perm[l]);
+  assert (forall k: int :: lo <= k && k <= hi ==> a[k] == old(a)[perm[k]]);
 }
 
